scratchpaper.v
@@ -1,0 +1,52 @@
+
+
+(*
+Conveluted Stackbased Implementation 
+ 
+Inductive RPN' : Set :=
+  | RPNlit' : lit -> RPN'
+  | RPNvar' : string -> RPN'
+  | RPNbinop' : (lit -> lit -> lit) -> RPN'
+.
+Fixpoint rpn' (e:Exp) {struct e} : list RPN' :=
+match e with
+| Elit l => RPNlit' l :: nil
+| Evar x => RPNvar' x :: nil
+| Eplus e1 e2 => rpn' e1 ++ rpn' e2 ++ RPNbinop' plus :: nil
+| Emin  e1 e2 => rpn' e1 ++ rpn' e2 ++ RPNbinop' min  :: nil
+| Emult e1 e2 => rpn' e1 ++ rpn' e2 ++ RPNbinop' mult :: nil
+end.
+Fixpoint rpn_eval' (inp: list RPN') (stack: list lit) (f : env) {struct inp} : option (list lit) :=
+match inp with
+| nil => Some stack
+| r::rs =>
+  match r with
+  | RPNlit' l => rpn_eval' rs (l::stack) f
+  | RPNvar' x => 
+    match f x with
+    | Some l  => rpn_eval' rs (l::stack) f
+    | _       => None
+    end
+  | RPNbinop' op =>
+    match stack with
+    | x::x'::xs => rpn_eval' rs ((op x x')::xs) f
+    | _ => None
+    end
+  end
+end.
+
+Lemma Equivalence_Eval_RPNEval' : forall e:Exp, eval e = rpn_eval' (rpn' e) nil.
+Proof.
+  induction e; simpl; try rewrite <- IHe1, <- IHe2; reflexivity.
+Qed.
+
+
+Definition rpn0':(list RPN') := (RPNlit' 1) :: (RPNlit' 2) :: (RPNbinop' plus)::nil.
+Eval compute in (rpn_eval' (rpn0') nil empty).
+Definition rpn1':(list RPN') := (RPNvar' "x") :: (RPNlit' 2) :: (RPNbinop' plus)::nil.
+Definition env0' := update empty "x" 4.
+Definition env1' := update env0 "y" 6.
+Eval compute in (rpn_eval' (rpn1') nil env0').
+Eval compute in (rpn_eval' (rpn1') nil empty).
+
+ *)
